function to memcpy a src vector into a from to to location in a dst vector, when the dst vector has sufficient space

lib/pulse/lib/Pulse.Lib.Array.fst
@@ -119,7 +119,87 @@ fn memcpy
   ()
 }
 
+let seq_append_lemma 
+  (#t:eqtype)
+  (s:Seq.seq t)
+  (ls:nat{ls == Seq.length s})
+  (from:nat {from < ls})
+  (k:nat{k < ls /\ k >= from})
+  : Lemma
+    (ensures Seq.equal s (Seq.append (Seq.append (Seq.slice s 0 from) (Seq.slice s from k)) (Seq.slice s k ls))) =
+  ()
 
+
+fn memcpy_from 
+ (#t:eqtype)
+        (l:SZ.t)
+        (src:larray t (SZ.v l))
+        (ldst:SZ.t)
+        (dst:larray t (SZ.v ldst))
+        (from:SZ.t {0 <= SZ.v from /\ (SZ.v l + SZ.v from) < SZ.v ldst })
+        (#p:perm)
+        (#src0 #dst0:Ghost.erased (Seq.seq t))
+  requires A.pts_to src #p src0 **
+           A.pts_to dst dst0
+  returns _:squash (Seq.length src0 == A.length src /\ Seq.length dst0 == A.length dst)
+  ensures A.pts_to src #p src0 **
+          A.pts_to dst (Seq.append (Seq.append (Seq.slice dst0 0 (SZ.v from)) src0) 
+                                         (Seq.slice dst0 (SZ.v from + SZ.v l) (SZ.v ldst)))
+{
+  pts_to_len src #p #src0;
+  pts_to_len dst #1.0R #dst0;
+  let mut i = 0sz;
+   let mut i = 0sz;
+  while (let vi = !i; (vi < l) )
+  invariant b. exists* (vi:US.t) (s:Seq.seq t). ( 
+    R.pts_to i vi **
+    A.pts_to src #p src0 **
+    A.pts_to dst s **
+    pure (vi <= l
+       /\ Seq.length s == Seq.length dst0
+       /\ (b == (vi < l))
+       /\ (forall (j:nat). j < SZ.v from ==> Seq.index s j == Seq.index dst0 j)
+       /\ (forall (j:nat). j < US.v vi ==> Seq.index s (j + SZ.v from) == Seq.index src0 j)
+       /\ (forall (j:nat). j >= US.v vi /\ j < SZ.v l ==> Seq.index s (j + SZ.v from) == Seq.index dst0 (j + SZ.v from))
+       /\ (forall (j:nat). j >= (SZ.v l + SZ.v from) /\ j < SZ.v ldst ==> Seq.index s j == Seq.index dst0 j)
+       ))
+
+
+  {
+    let vi = !i;
+    let x = src.(vi);
+
+    with s. assert (A.pts_to dst s);
+    (dst.(vi + from) <- x);
+    i := vi + 1sz;
+  };
+  with s. assert (A.pts_to dst s);
+  assert_ (pure (forall (j:nat). j < SZ.v from ==> Seq.index s j == Seq.index dst0 j));
+  assert_ (pure (forall (j:nat). j < US.v l ==> Seq.index s (j + SZ.v from) == Seq.index src0 j));
+  assert_ (pure (forall (j:nat). j >= (SZ.v l + SZ.v from) /\ j < SZ.v ldst ==> Seq.index s j == Seq.index dst0 j));
+  assert_ (pure (Seq.equal (Seq.slice s 0 (SZ.v from)) (Seq.slice dst0 0 (SZ.v from))));
+  assert_ (pure (Seq.equal (Seq.slice src0 0 (SZ.v l)) (Seq.slice src0 0 (SZ.v l))));
+  
+  assert_ (pure (Seq.equal (Seq.slice s (SZ.v from) (SZ.v l + SZ.v from)) (Seq.slice src0 0 (SZ.v l))));
+  assert_ (pure (Seq.equal (Seq.slice src0 0 (SZ.v l)) src0));
+  assert_ (pure (Seq.equal (Seq.slice s (SZ.v from) (SZ.v l + SZ.v from)) src0));
+  assert_ (pure (Seq.equal (Seq.slice s (SZ.v from + SZ.v l) (SZ.v ldst)) (Seq.slice dst0 (SZ.v from + SZ.v l) (SZ.v ldst))));
+  assert_ (pure (Seq.equal s (Seq.slice s 0 (SZ.v ldst))));
+  assert_ (pure (SZ.v from < SZ.v ldst));
+ 
+  assert_ (pure ((SZ.v from + SZ.v l) < (SZ.v ldst) /\ ((SZ.v from + SZ.v l)) >= (SZ.v from)));
+  
+  seq_append_lemma s (SZ.v ldst) (SZ.v from) (SZ.v from + SZ.v l);
+  assert_ (pure (Seq.equal s (Seq.append (Seq.append (Seq.slice s 0 (SZ.v from)) 
+                                               (Seq.slice s (SZ.v from) (SZ.v from + SZ.v l))) 
+                                   (Seq.slice s (SZ.v from + SZ.v l) (SZ.v ldst)))));
+  
+  
+  assert_ (pure (Seq.equal s (Seq.append (Seq.append (Seq.slice dst0 0 (SZ.v from)) src0) 
+                                         (Seq.slice dst0 (SZ.v from + SZ.v l) (SZ.v ldst)))));
+  ()
+  
+}
 
 fn fill (#t:Type0) (l:US.t) (a:larray t (US.v l)) (v:t)
   requires A.pts_to a 's
